coqdoc for interp.v and fundamental.v; also, move some stuff in fundamental.v to interp.v

theories/fundamental.v
@@ -1,71 +1,26 @@
 From tutorial_popl20 Require Export typed compatibility interp.
 
-Definition interp_env `{heapG Σ} (Γ : gmap string ty)
-  (ρ : list (sem_ty Σ)) : gmap string (sem_ty Σ) := flip interp ρ <$> Γ.
-Instance: Params (@interp_env) 3 := {}.
+(** * The fundamental theorem of logical relations
+
+    The fundamental theorem of logical relations says that any
+    syntactically typed term is also semantically typed:
+
+    if [Γ ⊢ e : τ] then [interp Γ ρ ⊨ e : 〚τ〛 ρ]
+
+    where [ρ] is any mapping free type variables in [Γ] and [τ] to
+    semantic types.
+
+    This theorem essentially follows from the compatibility lemmas by
+    a straightforward induction on the typing derivation.  *)
 
 Section fundamental.
   Context `{heapG Σ}.
   Implicit Types Γ : gmap string ty.
   Implicit Types τ : ty.
   Implicit Types ρ : list (sem_ty Σ).
-  Implicit Types i n j : nat.
 
-  Global Instance interp_ne τ : NonExpansive ⟦ τ ⟧.
-  Proof. induction τ; solve_proper. Qed.
-  Global Instance interp_proper τ : Proper ((≡) ==> (≡)) ⟦ τ ⟧.
-  Proof. apply ne_proper, _. Qed.
-
-  Lemma interp_env_empty ρ : interp_env (∅ : gmap string ty) ρ = ∅.
-  Proof. by rewrite /interp_env fmap_empty. Qed.
-  Lemma lookup_interp_env Γ x τ ρ :
-    Γ !! x = Some τ → interp_env Γ ρ !! x = Some (⟦ τ ⟧ ρ).
-  Proof. intros Hx. by rewrite /interp_env lookup_fmap Hx. Qed.
-  Lemma interp_env_binder_insert Γ x τ ρ :
-    interp_env (binder_insert x τ Γ) ρ
-    = binder_insert x (⟦ τ ⟧ ρ) (interp_env Γ ρ).
-  Proof. destruct x as [|x]=> //=. by rewrite /interp_env fmap_insert. Qed.
-
-  Lemma interp_ty_lift n τ ρ :
-    n ≤ length ρ →
-    ⟦ ty_lift n τ ⟧ ρ ≡ ⟦ τ ⟧ (delete n ρ).
-  Proof.
-    (* Use [elim:] instead of [induction] so we can properly name hyps *)
-    revert n ρ. elim: τ; simpl; try (intros; done || f_equiv/=; by auto).
-    - intros x n ρ ?. repeat case_decide; simplify_eq/=; try lia.
-      + by rewrite lookup_delete_lt.
-      + by rewrite lookup_delete_ge; last lia.
-    - intros τ IH n ρ ?. f_equiv=> A /=. naive_solver auto with lia.
-    - intros τ IH n ρ ?. f_equiv=> A /=. naive_solver auto with lia.
-  Qed.
-
-  Lemma interp_env_ty_lift n Γ ρ :
-    n ≤ length ρ →
-    interp_env (ty_lift n <$> Γ) ρ ≡ interp_env Γ (delete n ρ).
-  Proof.
-    intros. rewrite /interp_env -map_fmap_compose.
-    apply map_fmap_equiv_ext=> x A _ /=. by rewrite interp_ty_lift.
-  Qed.
-
-  Lemma interp_ty_subst i τ τ' ρ :
-    i ≤ length ρ →
-    ⟦ ty_subst i τ' τ ⟧ ρ ≡ ⟦ τ ⟧ (take i ρ ++ ⟦ τ' ⟧ ρ :: drop i ρ).
-  Proof.
-    (* Use [elim:] instead of [induction] so we can properly name hyps *)
-    revert i τ' ρ. elim: τ; simpl; try (intros; done || f_equiv/=; by auto).
-    - intros x i τ' ρ ?. repeat case_decide; simplify_eq/=; try lia.
-      + rewrite lookup_app_l; last (rewrite take_length; lia).
-        by rewrite lookup_take; last lia.
-      + by rewrite list_lookup_middle; last (rewrite take_length; lia).
-      + rewrite lookup_app_r; last (rewrite take_length; lia).
-        rewrite take_length lookup_cons_ne_0; last lia.
-        rewrite lookup_drop. do 2 f_equiv; lia.
-    - intros τ IH i τ' ρ ?. f_equiv=> A /=. rewrite IH /=; last lia.
-      by rewrite interp_ty_lift; last lia.
-    - intros τ IH i τ' ρ ?. f_equiv=> A /=. rewrite IH /=; last lia.
-      by rewrite interp_ty_lift; last lia.
-  Qed.
-
+  (* I'm not sure where I should move the following but they don't
+  seem to belong here! *)
   Instance ty_unboxed_sound τ ρ : ty_unboxed τ → SemTyUnboxed (⟦ τ ⟧ ρ).
   Proof. destruct 1; simpl; apply _. Qed.
   Instance ty_un_op_sound op τ σ ρ :
