theories/interp.v
@@ -1,4 +1,4 @@
-From tutorial_popl20 Require Export sem_type_formers types.
+From tutorial_popl20 Require Export sem_typed sem_type_formers types.
 
 (** * Here we use semantic type formers to define semantics of syntactic types.
 
@@ -21,3 +21,81 @@ Fixpoint interp `{heapG Σ} (τ : ty) (ρ : list (sem_ty Σ)) : sem_ty Σ :=
 where "⟦ τ ⟧" := (interp τ).
 
 Instance: Params (@interp) 2 := {}.
+
+(** Given a syntactic typing context [Γ] (a mapping from variables
+(string) to types) together with a mapping (represented as a list)
+from type variables (that appear freely in [Γ]) to their corresponding
+semantic types, we define a semantic typing context, i.e., a mapping
+from  variables (strings) to semantic types. *)
+Definition interp_env `{heapG Σ} (Γ : gmap string ty)
+  (ρ : list (sem_ty Σ)) : gmap string (sem_ty Σ) := flip interp ρ <$> Γ.
+Instance: Params (@interp_env) 3 := {}.
+
+(** Below we prove several useful lemmas about [interp] and
+    [interp_env] including important lemmas about the effect that
+    lifting (de Bruij indices) and substitution in type level
+    variables have on the interpretation of syntactic types and typing
+    contexts. *)
+Section interp_properties.
+  Context `{heapG Σ}.
+  Implicit Types Γ : gmap string ty.
+  Implicit Types τ : ty.
+  Implicit Types ρ : list (sem_ty Σ).
+  Implicit Types i n j : nat.
+
+  Global Instance interp_ne τ : NonExpansive ⟦ τ ⟧.
+  Proof. induction τ; solve_proper. Qed.
+  Global Instance interp_proper τ : Proper ((≡) ==> (≡)) ⟦ τ ⟧.
+  Proof. apply ne_proper, _. Qed.
+
+  Lemma interp_env_empty ρ : interp_env (∅ : gmap string ty) ρ = ∅.
+  Proof. by rewrite /interp_env fmap_empty. Qed.
+  Lemma lookup_interp_env Γ x τ ρ :
+    Γ !! x = Some τ → interp_env Γ ρ !! x = Some (⟦ τ ⟧ ρ).
+  Proof. intros Hx. by rewrite /interp_env lookup_fmap Hx. Qed.
+  Lemma interp_env_binder_insert Γ x τ ρ :
+    interp_env (binder_insert x τ Γ) ρ
+    = binder_insert x (⟦ τ ⟧ ρ) (interp_env Γ ρ).
+  Proof. destruct x as [|x]=> //=. by rewrite /interp_env fmap_insert. Qed.
+
+  Lemma interp_ty_lift n τ ρ :
+    n ≤ length ρ →
+    ⟦ ty_lift n τ ⟧ ρ ≡ ⟦ τ ⟧ (delete n ρ).
+  Proof.
+    (* Use [elim:] instead of [induction] so we can properly name hyps *)
+    revert n ρ. elim: τ; simpl; try (intros; done || f_equiv/=; by auto).
+    - intros x n ρ ?. repeat case_decide; simplify_eq/=; try lia.
+      + by rewrite lookup_delete_lt.
+      + by rewrite lookup_delete_ge; last lia.
+    - intros τ IH n ρ ?. f_equiv=> A /=. naive_solver auto with lia.
+    - intros τ IH n ρ ?. f_equiv=> A /=. naive_solver auto with lia.
+  Qed.
+
+  Lemma interp_env_ty_lift n Γ ρ :
+    n ≤ length ρ →
+    interp_env (ty_lift n <$> Γ) ρ ≡ interp_env Γ (delete n ρ).
+  Proof.
+    intros. rewrite /interp_env -map_fmap_compose.
+    apply map_fmap_equiv_ext=> x A _ /=. by rewrite interp_ty_lift.
+  Qed.
+
+  Lemma interp_ty_subst i τ τ' ρ :
+    i ≤ length ρ →
+    ⟦ ty_subst i τ' τ ⟧ ρ ≡ ⟦ τ ⟧ (take i ρ ++ ⟦ τ' ⟧ ρ :: drop i ρ).
+  Proof.
+    (* Use [elim:] instead of [induction] so we can properly name hyps *)
+    revert i τ' ρ. elim: τ; simpl; try (intros; done || f_equiv/=; by auto).
+    - intros x i τ' ρ ?. repeat case_decide; simplify_eq/=; try lia.
+      + rewrite lookup_app_l; last (rewrite take_length; lia).
+        by rewrite lookup_take; last lia.
+      + by rewrite list_lookup_middle; last (rewrite take_length; lia).
+      + rewrite lookup_app_r; last (rewrite take_length; lia).
+        rewrite take_length lookup_cons_ne_0; last lia.
+        rewrite lookup_drop. do 2 f_equiv; lia.
+    - intros τ IH i τ' ρ ?. f_equiv=> A /=. rewrite IH /=; last lia.
+      by rewrite interp_ty_lift; last lia.
+    - intros τ IH i τ' ρ ?. f_equiv=> A /=. rewrite IH /=; last lia.
+      by rewrite interp_ty_lift; last lia.
+  Qed.
+
+End interp_properties.
